Preservation proof:
Fixed bugs with Parameter/Variable P, formalized full selection case.

preservation.v
@@ -21,76 +21,64 @@ Section Preservation.
   Definition ftypeP := ftype P.
   Definition t_frame1' := t_frame1 P.
   Definition WF_Frame' := WF_Frame P.
+
+  Definition Reduction_SF' := Reduction_SF P.
+  Definition fieldsP := fields P.
+  Definition TypeChecksP := TypeChecks P.
+  Definition Heap_okP := Heap_ok P.
+  
+  
   
   Theorem preservation_light :
     forall gamma H H' L L' t t' sigma eff,
-      Reduction_SF ( # H, L, t !)
+      Reduction_SF' ( # H, L, t !)
                    ( # H', L', t' !)
       ->
-      TypeChecks gamma eff t sigma ->
-      {Gamma' : Gamma_type & TypeChecks Gamma' eff t' sigma}.
+      TypeChecksP gamma eff t sigma ->
+      {Gamma' : Gamma_type & TypeChecksP Gamma' eff t' sigma}.
     intros.
     case_eq t; intros;  rewrite H0 in *  ;    clear H0 t; inversion X;
     inversion X0;
-      exists (p_gamma.updatePartFunc gamma v sigma0); cbn;
-      rewrite H9 in *; auto.
+    exists (p_gamma.updatePartFunc gamma v sigma0); cbn;
+    rewrite H9 in *; auto.
   Qed.
 
   Local Open Scope type_scope.
 
-  
 
-  Theorem single_frame_WF_ENV_preservation :
-    forall H H' L L' t t' sigma ann,
-      WF_Frame' H (ann_frame (sframe L t) ann) sigma ->
-      Heap_ok H ->
-      Reduction_SF ( # H, L, t !) ( # H', L', t' !) ->
-      (WF_Frame' H' (ann_frame (sframe L' t') ann) sigma) *
-      (Heap_ok H').
+  Theorem preservation_case_var :
+    forall H L x y t sigma ann envVar,
+      WF_Frame' H (ann_frame (sframe L (t_let x <- Var y t_in (t))) ann) sigma ->
+      p_env.func L y = Some envVar ->
+      isTerm t ->
+      WF_Frame' H (ann_frame (sframe (p_env.updatePartFunc L x envVar) t) ann) sigma.
     intros.
-    rename H0 into asm0.
-    case_eq t; intros;   rewrite H0 in *  ;    clear H0 t;   inversion X0.
-
-    rewrite <- H7 in *; clear H7 H1 H0.
-    rewrite <- H8 in *; clear H2 L0 H8.
-    rewrite <- H6 in *; rewrite <- H9 in *; clear  H9 H6.
-    rewrite <- H5 in *; clear H5.
-    rewrite <- H4 in *; clear H4.
-
-    (* inversion H16. *)
-    (* rewrite H2 in *; clear H2 H16 H5. *)
-    (* rewrite <- H4 in *. *)
-    (* clear H15 H4 v. *)
-    (* clear L1 H11 t0 y0 x0. *)
-    (* assert (Some null_ref_box0 = Some null_ref_box). transitivity (p_env.func L y). *)
-    (* auto. auto. *)
-    (* inversion H1. *)
-    (* rewrite H4 in *. *)
-    (* clear H4 H1 H8 H21 null_ref_box0. *)
+    rename H0 into H10.
+    rename H1 into H3.
 
     inversion X.
     clear H5 t0. clear H4 H1 H2 H6 L0 ann0 sigma0 H0. 
     
-    inversion X1.
+    inversion X0.
     clear gamma H0 x0 H4 eff0 H1 t0 H6 H2 tau H5 e.
-    split.
+    (* split. *)
     apply (t_frame1' H (p_gamma.updatePartFunc Gamma x sigma0) eff t
-                    (p_env.updatePartFunc L x null_ref_box) ann sigma H3).
-    apply X4.
+                     (p_env.updatePartFunc L x envVar) ann sigma H3).
+    exact X3.
     split.
-    destruct X2.
+    destruct X1.
     apply (subset_preserved _ _ _ _ _ g).
     intros.
     elim (v_eq_dec x x0).
     intro; rewrite <- a in *; clear a.
 
-    inversion X3.
+    inversion X2.
     clear H6 H4 H1; rewrite <- H2 in *; clear H2 sigma2.
-    set (wf_var_y := snd X2 y sigma0 H5).
+    set (wf_var_y := snd X1 y sigma0 H5).
     
     (* 3.
      *)
-    induction null_ref_box.
+    induction envVar.
     (* 
      * 3. (a), L(y) = null
      *)
@@ -131,35 +119,13 @@ Section Preservation.
     auto.
 
     destruct b; destruct x2; destruct y0; destruct a; destruct H2.
-    (* induction b; destruct x2; induction p; destruct p; destruct H2. *)
 
     rewrite (_3_b_i_A) in *; inversion H1.
-    (* destruct H2. *)
-    (* rewrite ->  H8 in *. *)
-    (* clear o H8. *)
-    (* rename r into o. (* it couldn't do it directly *) *)
-    (* rename c into C'. *)
-    (* clear H1. *)
-
-    (* apply inr. *)
-    (* exists (C', o). *)
-    (* exists x2. *)
-    (* split. *)
-    (* apply p_env.updatedFuncProp; apply eq_refl. *)
-    (* split. *)
-
-    (* set (lem := proj1 (p_gamma.updatedFuncProp gamma  x sigma0 x) (eq_refl x)). *)
-    (* rewrite lem in H0; inversion H0. rewrite H6 in *. *)
-    (* rename sigma1 into sigma'; clear  H6 H0. *)
-    (* rewrite H2 in H5; inversion H5; rewrite <- H1 in *. *)
-    (* clear H1 H5. *)
-    (* exact lem. *)
-    (* exact H4. *)
 
     (* 3 c, L(y) = b(o)*)
     rename H10 into _3_c.
     rename r into o.
-    destruct X2 as [_3_c_i_A _3_c_i_B].
+    destruct X1 as [_3_c_i_A _3_c_i_B].
     clear Gamma.
     rename H5 into _1_b.
     rename sigma0 into sigma'.
@@ -214,7 +180,7 @@ Section Preservation.
     symmetry.
     apply p_gamma.updatedFuncProp. firstorder.
 
-    destruct X2 as [ _4_c_i _4_c_ii].
+    destruct X1 as [ _4_c_i _4_c_ii].
     set (_4_d := _4_c_ii z tau _4_a).
     unfold WF_Var.
     rewrite H0.
@@ -226,9 +192,9 @@ Section Preservation.
 
     set (lem''' := _4_c_i z _4_ca).
     case_eq (p_env.func L z).
-    intros envVar _4_ca_ii.
+    intros envVar' _4_ca_ii.
 
-    assert (p_env.func (p_env.updatePartFunc L x null_ref_box ) z = Some envVar) as _4_cb.
+    assert (p_env.func (p_env.updatePartFunc L x envVar ) z = Some envVar') as _4_cb.
     transitivity (p_env.func L z).
     apply p_env.updatedFuncProp. firstorder.
     exact _4_ca_ii.
@@ -241,26 +207,16 @@ Section Preservation.
     intro.
     set (lem'''':= proj2 (p_env.fDomainCompat L z ) H1).
     firstorder.
+  Qed.
 
-    apply asm0.
 
-    (* Case t = let y = Null in t' *)
-    rewrite  H9 in *; clear H9 e0 t H6.
-    rewrite <- H8 in *; clear H8.
-    rewrite <- H7 in *; clear H7 H'.
-    rewrite <- H5 in *; clear e H5.
-    rewrite <- H4 in *; clear H4.
-    clear H3 H1 L0 H0.
-    clear L'.
-    rename t' into t.
-
+  Theorem preservation_case_null :
+    forall H L t sigma ann x ,
+      WF_Frame' H (ann_frame (sframe L t_let x <- Null t_in (t)) ann) sigma ->
+      WF_Frame' H (ann_frame (sframe (p_env.updatePartFunc L x envNull) t ) ann) sigma.
+    intros.
     rename X into asm1.
-    rename asm0 into asm2.
-    rename X0 into asm0.
-    clear H2 . 
-
-    clear v.
-
+    
     inversion asm1.
     clear sigma0 ann0 H3 H5 t0 H4 H1 L0 H0 H2.
 
@@ -274,8 +230,7 @@ Section Preservation.
     rename X0 into _4_b.
 
     destruct _3_b as [_6_a _6_b].
-
-    split.
+    
     apply (t_frame1' H (p_gamma.updatePartFunc Gamma x sigma' )
                     eff t
                     (p_env.updatePartFunc L x envNull) ann sigma).
@@ -312,7 +267,7 @@ Section Preservation.
     
     (* rewrite H0. *)
     
-
+    
     
     (* Require Import Coq.Lists.List. *)
     assert (In z (p_gamma.domain Gamma)) as new_4_ca.
@@ -339,25 +294,25 @@ Section Preservation.
     intro.
     set (lem'''':= proj2 (p_env.fDomainCompat L z ) H0).
     firstorder.
-    exact asm2.
+  Qed.
 
-
-
-    (* Case let v = new C in t *)
-    rename X0 into asm1.
+  Theorem preservation_case_new :
+    forall H L sigma ann t C x o flds,
+      WF_Frame' H (ann_frame (sframe L t_let x <- New C t_in (t)) ann) sigma ->
+      Heap_okP H ->
+      ~ In o (p_heap.domain H) ->
+      isTerm t ->
+      fieldsP C flds ->
+      WF_Frame'
+        (p_heap.updatePartFunc H o (obj C (p_FM.newPartFunc flds FM_null)))
+        (ann_frame (sframe (p_env.updatePartFunc L x (envRef o)) t) ann) sigma.
+    intros.
     rename X into asm2.
-    rename asm0 into asm3.
-
-    (* 1 *)
-
-    rewrite -> H9 in *; clear H9 e0.
-    rewrite <- H6 in *; clear H6 t'.
-    rewrite <- H8  in *; clear L' H8.
-    rewrite <- H7 in *; clear H7 H'.
-    rewrite <- H4 in *; clear e H4.
-    rewrite <- H3 in *; clear H3 v.
-    clear H2 L0 H0 H1.
-    rewrite H12 in *; clear H12.
+    rename H2 into H5.
+    rename H0 into asm3.
+    rename H3 into H11.
+    rename H1 into H10.
+    
 
     (* 2 *)
     inversion asm2.
@@ -388,7 +343,7 @@ Section Preservation.
 
     (* section between 5, 6 let's call it half_6 *)
     (* This is not in the same order on paper *)
-    split.
+    (* split. *)
     apply ( t_frame1' _
                      (p_gamma.updatePartFunc Gamma x (typt_class C))
                      eff _ _ ann sigma).
@@ -531,81 +486,431 @@ Section Preservation.
     split.
     rewrite <- H1.
     apply (p_gamma.updatedFuncProp). firstorder.
+    admit. 
+    admit.
+    admit.
+    Admitted.
+
     
-    TODO finish here!
+  (*   P : Program *)
+  (* H : Heap_type *)
+  (* L : Env_type *)
+  (* sigma : typecheck_type *)
+  (* ann : annotation_type *)
+  (* t : ExprOrTerm *)
+  (* C : ClassName_type *)
+  (* x : VarName_type *)
+  (* asm2 : WF_Frame' H (ann_frame (sframe L t_let x <- New C t_in (t)) ann) *)
+  (*          sigma *)
+  (* asm3 : Heap_okP H *)
+  (* o : p_gamma.A *)
+  (* FM : p_FM.PartFunc *)
+  (* flds : list FieldName_type *)
+  (* asm1 : Reduction_SF' ( # H, L, t_let x <- New C t_in (t) ! ) *)
+  (*          ( # p_heap.updatePartFunc H o *)
+  (*                (obj C (p_FM.newPartFunc flds FM_null)), *)
+  (*          p_env.updatePartFunc L x (envRef o), t ! ) *)
+  (* H5 : isTerm t *)
+  (* H10 : ~ In o (p_heap.domain H) *)
+  (* H11 : fields reductions.P C flds *)
+  (* ============================ *)
+  (*  WF_Frame' *)
+  (*    (p_heap.updatePartFunc H o (obj C (p_FM.newPartFunc flds FM_null))) *)
+  (*    (ann_frame (sframe (p_env.updatePartFunc L x (envRef o)) t) ann) sigma * *)
+  (*  Heap_okP *)
+  (*    (p_heap.updatePartFunc H o (obj C (p_FM.newPartFunc flds FM_null))) *)
+
+  Theorem preservation_case_box :
+    forall H L sigma ann t C x o flds,
+      WF_Frame' H (ann_frame (sframe L t_let x <- Box C t_in (t)) ann) sigma ->
+      Heap_okP H ->
+      ~ In o (p_heap.domain H) ->
+      isTerm t ->
+      fieldsP C flds ->
+      WF_Frame'
+        (p_heap.updatePartFunc H o (obj C (p_FM.newPartFunc flds FM_null)))
+        (ann_frame (sframe (p_env.updatePartFunc L x (envBox o)) t) ann) sigma.
+    admit. Admitted.
+
+  Theorem preservation_case_select :
+    forall H L sigma ann x y f t C FM fmVal o,
+      WF_Frame' H (ann_frame (sframe L t_let x <- FieldSelection y f t_in (t)) ann) sigma ->
+      Heap_okP H ->
+      p_env.func L y = Some (envRef o) ->
+      p_heap.func H o = Some (obj C FM) ->
+      p_FM.func FM f = Some fmVal ->
+      isTerm t ->
+      WF_Frame'
+        H
+        (ann_frame (sframe (p_env.updatePartFunc L x (fm2env fmVal)) t) ann) sigma.
     intros.
-    exact i.
-    intros not_in dummy; clear dummy.
-    set (H'o'_is_none := proj1 ((p_heap.fDomainCompat 
-                    (p_heap.updatePartFunc H o (obj C (p_FM.newPartFunc flds FM_null)))
-                                ) o' ) not_in).
+
+    (* 2 *)
+    rename H1 into _2_ab.
+    rename H2 into _2_cd.
+    rename H3 into _2_e.
+    rename H4 into t_is_term.
+    rename H0 into _2_j.
+    rename X into _2_k.
+
+    (* 3 *)
+    inversion _2_k.
+    clear H3 sigma0 H5 ann0 H4 H1 H2.
+    rename X into _3_a.
+    rename X0 into _3_b.
+
+
+    (* 4 *)
+    inversion _3_a.
+    clear tau H3 H7 t1 H5 e H4 x0 eff0 H2.
+    rewrite <- H1 in * ; clear H1 Gamma.
+    inversion X.
+    clear H5 f0 H1 x0 eff0 H3 gamma0 H2.
+    rename C0 into D.
+    rename H7 into _4_a.
+    rename witn into _4_b.
+    set (E := ftype P D f _4_b).
+    rewrite <- H4 in *.
+    fold E in X, X0.
+    clear H4.
+    (* rename H4 into _4_c. *)
+    rename X0 into _4_d.
+    rename X into _4_e.
+    set (L' := p_env.updatePartFunc L x (fm2env fmVal)).
+    clear t0 L0 H0.
+
+
+    (* 5 *)
+    set (Gamma' := p_gamma.updatePartFunc gamma x (typt_class E)).
+    fold Gamma' in _4_d.
+    
+    (* 6 *)
+    inversion _3_b.
+    rename H0 into _3_b_i.
+    rename X into _3_b_ii.
+    set (_6 := subset_preserved gamma L x (typt_class E) (fm2env fmVal)  _3_b_i).
+
+
+    (* OTHER ORDER COMPARED TO paper proof*)
+    clear H6 sigma0.
+    apply (t_frame1 P _ Gamma' eff _ _ _ _ t_is_term _4_d).
+    split.
+    apply _6.
+    intros z tau.
+
+    (* END OTHER *)
+
+    case_eq (v_eq_dec x z).
+    (* 7 *)
+    (* 7 a *)
+    intros.
+    rewrite <- e in *; clear e z.
+    clear H0.
+    assert (p_env.func L' x = Some (fm2env fmVal)) as _7_a.
+    unfold L'.
+    rewrite  ( proj1 (p_env.updatedFuncProp L x (fm2env fmVal) x) (eq_refl x)).
+    reflexivity.
+    
+    assert (p_gamma.func Gamma' x = Some (typt_class E)) as gamma_x_E.
+    unfold Gamma'.
+    rewrite  ( proj1 (p_gamma.updatedFuncProp gamma x (typt_class E) x) (eq_refl x)).
+    reflexivity.
+    clear H1.
+
+    (* 7 b *)
+    induction fmVal; unfold fm2env in _7_a.
+    
+    (* 7 b i *)
+    apply inl. apply inl.
+    exact _7_a.
+
+    (* 7 c *)
+    rename r into o'.
+    set (test := _2_j o C FM _2_cd f o').
+    
+    Print Heap_obj_ok.
+    apply inl.  apply inr.
+    exists (E, o').
+    Print p_heap.fDomainCompat.
+    unfold Gamma'.
+    assert (subclass P C D) as C_sub_D.
+    
+    induction ( _3_b_ii y (typt_class D) _4_a).
+    induction a.
+    rewrite  _2_ab in a; discriminate a.
+    destruct b.
+    destruct x0.
+    destruct y0.
+    destruct a.
+    destruct H1.
+    rewrite _2_ab in H0.
+    inversion H0.
+    rewrite H4 in *.
+    rewrite _4_a in H1.
+    inversion H1.
+    rewrite <- H5 in *.
+    clear c H5.
+    assert (heap_typeof H r x0 = C).
+    unfold heap_typeof.
+    rewrite <- H4.
+    rewrite _2_cd.
+    reflexivity.
+    rewrite H3 in H2.
+    inversion H2.
+    exact H7.
+    destruct b.   destruct x0. 
+    destruct y0.
+    destruct a.
+    rewrite _2_ab in H0.
+    inversion H0.
+    
+    assert (fld P C f) as f_field_C.
+    apply (field_subclass P C D  _  _4_b).
+    
+    exact C_sub_D.
+    destruct (test f_field_C _2_e).
+    clear test.
+    exists x0.
+    split.
+    exact _7_a.
+    split.
+    exact gamma_x_E.
+    
+    (*  *)
+    (*
+     * know: Gamma' x = E
+     * typeof(H, o') <: ftype(C, f)
+     * --------------
+     * ftype(C, f) = E
+     * --------------------- 
+     * Goal:  heapof(H, o') <: E
+     *
+     *)
+    apply classSub.
+    assert (E = heap.ftypeP P C f f_field_C).
+    unfold E.
+    unfold heap.ftypeP.
+    rewrite (unique_ftype P C f f_field_C (field_subclass P C D f f_field_C C_sub_D)).
+    rewrite <- (ftype_subclass P C D f f_field_C C_sub_D).
+    apply (unique_ftype P D f _ _).
+    rewrite <- H0 in s.
+    exact s.
+
+    (* 8 *)
+    intros.
+    clear H0.
+
+    (* 8 a b *)
+    assert (p_gamma.func gamma z = Some tau).
+    rewrite <- H1.
+    symmetry.
+    set (lem := proj2 (p_gamma.updatedFuncProp gamma x (typt_class E) z)).
+    firstorder.
+    rename H0 into _8_b.
+    assert (In z (p_gamma.domain gamma)) as _8_a.
+    apply (p_gamma.in_part_func_domain _ z tau _8_b).
+
+    (* 8 c *)
+    assert (In z (p_env.domain L)) as _8_c.
+    apply (_3_b_i _ _8_a).
+
+    set (_8_e_i := _3_b_ii z tau _8_b).
+    unfold WF_Var.
+
+    assert (p_env.func L z = p_env.func L' z) as _8_d.
+    set (lem := proj2 (p_env.updatedFuncProp L x (fm2env fmVal) z)).
+    symmetry. firstorder.
+    rewrite <- _8_d.
+    rewrite <- _8_b in H1.
+    rewrite H1.
+    exact _8_e_i.
+  Qed.
+
+
+  Theorem single_frame_WF_ENV_preservation :
+    forall H H' L L' t t' sigma ann,
+      WF_Frame' H (ann_frame (sframe L t) ann) sigma ->
+      Heap_okP H ->
+      Reduction_SF' ( # H, L, t !) ( # H', L', t' !) ->
+      (WF_Frame' H' (ann_frame (sframe L' t') ann) sigma) *
+      (Heap_okP H').
+    intros.
+    rename H0 into asm0.
+    case_eq t; intros;   rewrite H0 in *  ;    clear H0 t;   inversion X0.
+
+    (* Case let x = y in t *)
+    
+    rewrite <- H7 in *; clear H7 H1 H0.
+    rewrite <- H8 in *; clear H2 L0 H8.
+    rewrite <- H6 in *; rewrite <- H9 in *; clear  H9 H6.
+    rewrite <- H5 in *; clear H5.
+    rewrite <- H4 in *; clear H4.
+    Check preservation_case_var.
+
+    split.
+    exact (preservation_case_var H L x y t sigma ann null_ref_box X H10 H3).
+    assumption.
+    
+    (* Case t = let y = Null in t' *)
+    
+    rewrite  H9 in *; clear H9 e0 t H6.
+    rewrite <- H8 in *; clear H8.
+    rewrite <- H7 in *; clear H7 H'.
+    rewrite <- H5 in *; clear e H5.
+    rewrite <- H4 in *; clear H4.
+    clear H3 H1 L0 H0.
+    clear L'.
+    rename t' into t.
+
+    rename X into asm1.
+    rename asm0 into asm2.
+    rename X0 into asm0.
+    clear H2 . 
+
+    clear v.
+
+    split.
+
+    exact (preservation_case_null H L t sigma ann x asm1).
+    exact asm2.
+
+
+    (* Case let v = new C in t *)
+
+    
+
+    
+    
+    rename X0 into asm1.
+    rename X into asm2.
+    rename asm0 into asm3.
+
+    (* 1 *)
+
+    rewrite -> H9 in *; clear H9 e0.
+    rewrite <- H6 in *; clear H6 t'.
+    rewrite <- H8  in *; clear L' H8.
+    rewrite <- H7 in *; clear H7 H'.
+    rewrite <- H4 in *; clear e H4.
+    rewrite <- H3 in *; clear H3 v.
+    clear H2 L0 H0 H1.
+    rewrite H12 in *; clear H12.
+
+    split.
+    Check preservation_case_new.
+    exact (preservation_case_new H L sigma ann t C x o flds asm2 asm3 H10 H5 H11).
+
+
+    (* intros. *)
+    (* exact i. *)
+    (* intros not_in dummy; clear dummy. *)
+    (* set (H'o'_is_none := proj1 ((p_heap.fDomainCompat  *)
+    (*                 (p_heap.updatePartFunc H o (obj C (p_FM.newPartFunc flds FM_null))) *)
+    (*                             ) o' ) not_in). *)
 
     
     
            
-    set (new_4d := _3_b z tau new_4_a).
-    unfold WF_Var in new_4d.
-    rewrite new_4_cb in *.
-    rewrite new__4_ca_ii in *.
-    rewrite new_4_a in *.
-    rewrite _6.
+    (* set (new_4d := _3_b z tau new_4_a). *)
+    (* unfold WF_Var in new_4d. *)
+    (* rewrite new_4_cb in *. *)
+    (* rewrite new__4_ca_ii in *. *)
+    (* rewrite new_4_a in *. *)
+    (* rewrite _6. *)
 
-    (* 6 a *)
-    induction envVar.
+    (* (* 6 a *) *)
+    (* induction envVar. *)
     
-    apply inl. apply inl. reflexivity.
-    case_eq (rn_eq_dec r o).
-    intros r_o_eq dummy'. clear dummy' dummy.
-    rewrite r_o_eq in *.
+    (* apply inl. apply inl. reflexivity. *)
+    (* case_eq (rn_eq_dec r o). *)
+    (* intros r_o_eq dummy'. clear dummy' dummy. *)
+    (* rewrite r_o_eq in *. *)
     
-    set (lemm := proj1 (p_heap.updatedFuncProp H o (obj C (p_FM.newPartFunc flds FM_null)) o)
-                         (eq_refl _)
-            ).
+    (* set (lemm := proj1 (p_heap.updatedFuncProp H o (obj C (p_FM.newPartFunc flds FM_null)) o) *)
+    (*                      (eq_refl _) *)
+    (*         ). *)
     
-    destruct new_4d.
-    destruct s.
-    inversion e.
-    destruct s.
-    destruct x0.
-    destruct y.
-    destruct a.
-    inversion H0.
-    rewrite -> H3 in *.
-    clear o H3.
-    rename r0 into o.
-    clear r_o_eq r.
-    clear H0.
-    destruct H1.
-    inversion H0.
-    rewrite -> H3 in *.
-    clear H3 tau.
-    clear H0.
+    (* destruct new_4d. *)
+    (* destruct s. *)
+    (* inversion e. *)
+    (* destruct s. *)
+    (* destruct x0. *)
+    (* destruct y. *)
+    (* destruct a. *)
+    (* inversion H0. *)
+    (* rewrite -> H3 in *. *)
+    (* clear o H3. *)
+    (* rename r0 into o. *)
+    (* clear r_o_eq r. *)
+    (* clear H0. *)
+    (* destruct H1. *)
+    (* inversion H0. *)
+    (* rewrite -> H3 in *. *)
+    (* clear H3 tau. *)
+    (* clear H0. *)
     
     
-    destruct s.
-    apply inl. apply inl.
-    exact e.
-    apply inl. apply inr.
-    destruct s.
-    destruct x0.
-    exists (c, r).
-    destruct y.
-    TODO FINISH!!!
-    intro.
-    set (lem'''':= proj2 (p_env.fDomainCompat L z ) H0).
-    firstorder.
+    (* destruct s. *)
+    (* apply inl. apply inl. *)
+    (* exact e. *)
+    (* apply inl. apply inr. *)
+    (* destruct s. *)
+    (* destruct x0. *)
+    (* exists (c, r). *)
+    (* destruct y. *)
+    (* TODO FINISH!!! *)
+    (* intro. *)
+    (* set (lem'''':= proj2 (p_env.fDomainCompat L z ) H0). *)
+    (* firstorder. *)
     
     
         
-    (* Section half_6 from paper: *)
+    (* (* Section half_6 from paper: *) *)
     
-    assert (p_env.updatePartFunc L x (envRef o) )
-    
-    
-                     Gamma eff t L ann sigma,)
-    
-    set (_2_A := t)
+    (* assert (p_env.updatePartFunc L x (envRef o) ) *)
     
     
+    (*                  Gamma eff t L ann sigma,) *)
     
+    (* set (_2_A := t) *)
+    admit.
+    
+    
+    
+    (* Case let x = Box C in t*)
+    Check    preservation_case_box.
+    split.
+    rewrite <- H6 in *; clear H6.
+    rewrite <- H9 in *; clear H9 t' e0.
+    rewrite <- H8 in *; clear H8 L'.
+    rewrite <- H7 in *; clear H7 H'.
+    rewrite <- H4 in *; clear e H4.
+    rewrite <- H3 in *; clear H3 v.
+    clear H2 L0 H1 H0.
+    rewrite H12 in *; clear H12 FM.
+    apply (preservation_case_box H L sigma ann t C x o flds X asm0 H10 H5 H11).
+    admit.
+
+
+
+    (* Case SELECT, let x = y.f in t *)
+    split.
+
+    rewrite <- H6 in *; clear H6 e0.
+    rewrite <- H9 in *; clear H9 t'.
+    rewrite <- H8 in *; clear H8 L'.
+    rewrite <- H7 in *; clear H7 H'.
+    rewrite <- H4 in *; clear H4 e.
+    rewrite <- H3 in *; clear H3 v.
+    clear L0 H0 H2 H1.
+    Check preservation_case_select.
+    apply (preservation_case_select H L sigma ann x y f t C FM fmVal o X asm0 H10 H11 H12 H5).
+    rewrite <- H7; exact asm0.
+
+    (* Case ASSIGN, let x = (y.f = z) in t *)
+    admit.
+    Admitted.
+
+
+  
     
